Theorem
> Let $S_n$ be the sum of the first $n$ positive integers. That is, $S_n = \sum\limits_{i=1}^{n} i$

$S_3 = 1 + 2 + 3 = 6 = \sum\limits_{i=1}^{3} i$


Proposition
>$P(n) = S_n = \dfrac{n(n+1)}{2}$

Prove
>$P(n+1) = S_{n+1} = \dfrac{n(n+1)}{2}$

<br/><br/>
Basic Step
> Let $n=3$
> $S_3 = \dfrac{3(3+1)}{2} $
> $ = \dfrac{12}{2} = 6$

<br/><br/>
Induction Step

> $S_n = \sum\limits_{i=1}^{n} i = \dfrac{n(n+1)}{2}$

<br/>

>$S_{n+1} = \sum\limits_{i=1}^{n+1}i$

>$ = \sum\limits_{i=1}^{n}i + (n+1)$

>$ = \dfrac{n(n+1)}{2} + (n+1)$

>$ = \dfrac{n(n+1)}{2} + \dfrac{2(n+1)}{2}$

>$ = \dfrac{n(n+1) + 2(n+1)}{2}$

>$ = \dfrac{n^2+3n+2}{2}$




<br/><br/><br/><br/><br/><br/><br/><br/>